More fiddles with layout for classes.  Think I have something that's roughly right.  Need to function dispatch next.

holsrcs/class_infoScript.sml
@@ -9,12 +9,14 @@ open boolSimps
 
 (* Standard HOL ancestory theories *)
 open arithmeticTheory pred_setTheory integerTheory
-local open wordsTheory integer_wordTheory finite_mapTheory in end
+local
+  open wordsTheory integer_wordTheory finite_mapTheory containerTheory
+in end
 
 (* C++ ancestor theories  *)
 open statesTheory
 
-val _ = new_theory "hierarchy";
+val _ = new_theory "class_info";
 
 (* BAD_ASSUMPTION: for the moment, our hierarchies only allow one
    ancestor class at most
@@ -47,12 +49,31 @@ val (rsubobjs_rules, rsubobjs_ind, rsubobjs_cases) = Hol_reln`
       rsubobjs s (C, C::Cs))
 `;
 
+val calc_rsubobjs = store_thm(
+  "calc_rsubobjs",
+  ``(C,Cs) IN rsubobjs s =
+       (Cs = [C]) /\ C IN FDOM (deNONE s.classmap) \/
+       ?D Cs'. s |- C < D /\ (D,Cs') IN rsubobjs s /\
+                 (Cs = C::Cs')``,
+  SRW_TAC [][SPECIFICATION] THEN
+  CONV_TAC (LAND_CONV (ONCE_REWRITE_CONV [rsubobjs_cases])) THEN
+  SRW_TAC [][SPECIFICATION] THEN
+  METIS_TAC [])
+
 (* The Subobjs relation of Wasserab et al.  Because of the absence of
    multiple inheritance, let alone virtual (shared) ancestors, this is
    currently the same as rsubobjs *)
 val (subobjs_rules, subobjs_ind, subobjs_cases) = Hol_reln`
   (!C Cs s. rsubobjs s (C,Cs) ==> subobjs s (C,Cs))
 `;
+
+val calc_subobjs = store_thm(
+  "calc_subobjs",
+  ``(C,Cs) IN subobjs s = (C,Cs) IN rsubobjs s``,
+  SRW_TAC [][SPECIFICATION] THEN
+  CONV_TAC (LAND_CONV (ONCE_REWRITE_CONV [subobjs_cases])) THEN
+  SRW_TAC [][]);
+
 
 val pord1_def = Define`
   pord1 (s, C) Cs Ds = (Cs = FRONT Ds) /\ (C,Cs) IN rsubobjs s /\
@@ -146,10 +167,114 @@ val nsdmembers_def = Define`
               cinfo.fields)
 `
 
+(* p is the set of all the subobjs for a given class *)
+val class_layout_def = Define`
+  class_layout (p : string list set) = SET_TO_LIST p
+`
+
+val class_layout_SING = store_thm(
+  "class_layout_SING",
+  ``class_layout {p} = [p]``,
+  SRW_TAC [][class_layout_def, containerTheory.SET_TO_LIST_THM, CHOICE_SING])
+val _ = export_rewrites ["class_layout_SING"]
+
+(* This can be passed to the sizeof relation in order to calculate the size
+   and offset information for classes.  *)
+(* BAD_ASSUMPTION:
+     this doesn't allow for the inclusion of vptr entries in classes
+*)
+val class_elems_def = Define`
+  class_elems s =
+    FUN_FMAP (\c. FLAT (MAP (\cpath. THE (nsdmembers s (LAST cpath)))
+                            (class_layout { so | (c,so) IN subobjs s })))
+             (FDOM s.classmap)
+`
+
+(* SANITY *)
+val class_elems_example1 = store_thm(
+  "class_elems_example1",
+  ``class_elems
+       <| classmap :=
+             FEMPTY |+
+               ("c",
+                SOME <| fields := [(FldDecl "foo" (Unsigned Int), F, Public);
+                                   (FldDecl "bar" Bool, T, Public);
+                                   (FldDecl "d" (Class "d"), F, Private);
+                                   (FldDecl "baz" BChar, F, Public)];
+                        ancestors := NONE |>) |+
+               ("d",
+                SOME <| fields := [(FldDecl "q" (Signed Int), F, Public)];
+                        ancestors := NONE |>) |> ' "c" =
+       [("foo", Unsigned Int); ("d", Class "d"); ("baz", BChar)]``,
+  SRW_TAC [][finite_mapTheory.FLOOKUP_UPDATE, nsdmembers_def,
+             ancestor_def, class_elems_def, calc_subobjs,
+             Once calc_rsubobjs, finite_mapTheory.FUN_FMAP_DEF,
+             finite_mapTheory.FAPPLY_FUPDATE_THM]);
+
+(* SANITY *)
+val class_elems_example2 = store_thm(
+  "class_elems_example2",
+  ``class_elems
+       <| classmap :=
+             FEMPTY |+
+               ("c",
+                SOME <| fields := [(CFnDefn Bool "f" [] (Block F [][]), F,
+                                    Public);
+                                   (FldDecl "bar" Bool, T, Public)];
+                        ancestors := SOME "d" |>) |+
+               ("d",
+                SOME <| fields := [(FldDecl "q" (Signed Int), F, Public)];
+                        ancestors := NONE |>) |> ' "c" =
+       [("q", Signed Int)]``,
+  SRW_TAC [][finite_mapTheory.FLOOKUP_UPDATE,
+             ancestor_def, class_elems_def, calc_subobjs,
+             Once calc_rsubobjs, finite_mapTheory.FUN_FMAP_DEF,
+             finite_mapTheory.FAPPLY_FUPDATE_THM] THEN
+  ONCE_REWRITE_TAC [calc_rsubobjs] THEN
+  SRW_TAC [][ancestor_def, GSPEC_OR, INSERT_UNION_EQ] THEN
+  Q.SUBGOAL_THEN `!x y. ~(x = y) ==> ((class_layout {x;y} = [x;y]) \/
+                                      (class_layout {x;y} = [y;x]))`
+    (Q.SPECL_THEN [`["c"]`, `["c"; "d"]`] MP_TAC)
+  THENL [
+    SRW_TAC [][class_layout_def] THEN
+    SRW_TAC [][containerTheory.SET_TO_LIST_THM] THEN
+    SRW_TAC [CONJ_ss][REST_DEF, DELETE_INSERT] THEN
+    SRW_TAC [][containerTheory.SET_TO_LIST_THM, CHOICE_SING] THEN
+    Q.ISPEC_THEN `{x:string list;y}` MP_TAC CHOICE_DEF THEN SRW_TAC [][],
+    ALL_TAC
+  ] THEN
+  SRW_TAC [][] THEN
+  SRW_TAC [][nsdmembers_def, finite_mapTheory.FLOOKUP_UPDATE]);
+
+
+(* ---------------------------------------------------------------------- *)
+
+(* looking up a field's information (type and index) requires a map from
+   class name to (name#type) list.   This is the lookup function that only
+   returns fields and not functions *)
+(* BAD_ASSUMPTION: this doesn't handle masking of names properly *)
+val lfimap_def = Define`
+  lfimap s = class_elems s
+`;
 
 
 
+(* BAD ASSUMPTION: no classes are abstract *)
+(* type-checking requires a variety of pieces of information, which we derive
+   from a state with this function *)
+val expr_type_comps_def = Define`
+  expr_type_comps s =
+    <| class_fields := lfimap s;
+       var_types := s.typemap ;
+       abs_classes := {} |>
+`;
 
+(* sizeof calculations expect to find a map from class name to a list
+   of types (the class's (non-static) fields.  This function calculates
+   that map from a classmap *)
+val sizeofmap_def = Define`
+  sizeofmap s = MAP SND o_f lfimap s
+`;
 
 
 
